refactor: Explicitly track which (linear) variables have become stale
This PR refactors a context to be a list of _optional_ types, where a particular entry being `none` means that the corresponding variable was linear and has been used already.

This replaces the previous mechanism, where linear variables were completely erased from the context, which in turn meant that the De Bruijn indices of linear variable were getting reused.

EffectSSA/Types/Context/TVarList.lean
@@ -32,6 +32,9 @@ unifying them.
 /--
 `vs : TVarList Γ Δ` is a list of variables,
 such that `vs[i]` is assigned the respective type `Δ[i]` in `Γ`.
+
+Note that this includes that if `Δ[i]` is stale, the corresponding variable
+`vs[i]` is required to be stale, too.
 -/
 structure TVarList (Γ : Context τ) (Δ : Context τ) where
   toList : List Var
@@ -69,9 +72,7 @@ def asHom (vs : TVarList Γ Δ) : Δ.Hom Γ where
   raw v := vs.toList[v.toNat]?.getD v
   ty_eq := by
     intro v t (hv : _ = some _)
-    have := vs.wt ⟨v.toNat, by
-      change Δ.toList[v.toNat]? = _ at hv
-      grind⟩
+    have := vs.wt ⟨v.toNat, by grind⟩
     grind
 
 /--
@@ -87,15 +88,16 @@ abbrev get (vs : TVarList Γ Δ) : TVar Δ t → TVar Γ t :=
 Map a function into a non-dependent type `α` over a TVarList, yielding a regular
 (homogeneous) list.
 
-Note that the function is _only_ applied to variables which are live, according
-to `Δ`, any stale variables are ignored.
+Note that the function is _only_ applied to variables which are live,
+any stale variables are mapped to `none` in the resulting list.
 -/
-def map (f : ∀ {t}, TVar Γ t → α) (vs : TVarList Γ Δ) : List α :=
-  Δ.toList.zipIdx.attach.map fun ⟨⟨t, i⟩, h⟩ =>
-    let v : TVar Δ t := ⟨.ofNat i, by
-      show Δ.toList[i]? = some t
-      grind⟩
-    f (vs.get v)
+def map (f : ∀ {t}, TVar Γ t → α) (vs : TVarList Γ Δ) : List (Option α) :=
+  Δ.toList.zipIdx.attach.map fun ⟨⟨t?, i⟩, h⟩ =>
+    t?.attach.map fun ⟨t, ht⟩ =>
+      let v : TVar Δ t := ⟨.ofNat i, by
+        show Δ.toList[i]?.join = some t
+        grind⟩
+      f (vs.get v)
 
 /-!
 ## Lemmas
@@ -104,19 +106,21 @@ def map (f : ∀ {t}, TVar Γ t → α) (vs : TVarList Γ Δ) : List α :=
 section Lemmas
 variable {ts} (f : ∀ {t}, TVar Γ t → α) (vs : TVarList Γ Δ)
 
-@[simp] theorem length_map : (vs.map f).length = Δ.size := by
+attribute [grind =] List.mk_mem_zipIdx_iff_getElem?
+
+@[simp, grind =] theorem length_map : (vs.map f).length = Δ.size := by
   simp [map]
 
 @[grind =]
 theorem getElem?_map (i : Nat) :
     (vs.map @f)[i]? =
       let i := Var.ofNat i
-      if hi : i.InBounds Δ then
-        some <| @f Δ[i] <| vs.get ⟨i, by grind⟩
+      if hi : i.LiveIn Δ then
+        some <| some <| @f Δ[i] <| vs.get ⟨i, by grind⟩
+      else if i.toNat < Δ.size then
+        some none
       else
         none := by
-  by_cases hi : (Var.ofNat i).InBounds Δ
-  · grind [map]
-  · simp [hi]; grind
+  grind [map, Var.LiveIn, Context.get?]
 
 end Lemmas
